% chktex-file 1 chktex-file 8 chktex-file 9 chktex-file 12 chktex-file 13 chktex-file 15 chktex-file 17 chktex-file 18 chktex-file 26 chktex-file 31 chktex-file 36 chktex-file 44
\documentclass[10pt]{article}
\input{/Users/mr.hassium/Desktop/Github/Hello-World/hassium.tex}
\def\htitle{Elementary Differential Geometry}
\def\hauthor{Hassium}\let\hfauthor\hauthor
\begin{document}
\hsetup
\htoc
\hmain
\par
\section{Calculus on Euclidean Space}
% 1.1 Euclidean Space
\begin{definition}
    The \hdef{Euclidean 3-space}, denoted ${\R}^{3}$, is the set of ordered triples of the form $p=({p}_{1},{p}_{2},{p}_{3})$, where ${p}_{i}\in\R$. An element of ${\R}^{3}$ is called a \hdef{point}.
\end{definition}
\par
Let $p=({p}_{1},{p}_{2},{p}_{3}),q=({q}_{1},{q}_{2},{q}_{3})\in{\R}^{3}$ and let $a\in\R$. Define the addition to be $p+q=({p}_{i}+{q}_{i})$ and define the scalar multiplication to be $ap=(a{p}_{i})$. The additive identity $0=(0,0,0)$ is called the \hdef{origin} of ${\R}^{3}$. It is trivial that ${\R}^{3}$ is a vector space over $\R$.
\begin{definition}
    Let $x$, $y$, and $z$ be real-valued functions on ${\R}^{3}$ such that for all $p=({p}_{1},{p}_{2},{p}_{3})\in{\R}^{3}$, $x(p)={p}_{1}$. $y(p)={p}_{2}$, and $z(p)={p}_{3}$. We call $x$, $y$, and $z$ the \hdef{natural coordinate functions} of ${\R}^{3}$.
\end{definition}
\par
Let $x$, $y$, and $z$ be the natural coordinate functions, rewrite $x={x}_{1}$, $y={x}_{2}$, and $z={x}_{3}$. Then we have $p=({p}_{i})=({x}_{i}(p))$.
\begin{definition}
    A real-valued function $f$ on ${\R}^{3}$ is \hdef{differentiable} if all partial derivatives exist and continuous.
\end{definition}
\par
Let $x=({x}_{1},{x}_{2},{x}_{3})\in{\R}^{3}$, we define the norm to be $\norm{x}=\sqrt{\sum{{x}_{i}}^{2}}$.
\begin{definition}
    A subset $O\sub{\R}^{3}$ is \hdef{open} if for all $p\in O$, there exists $\ve>0$ such that $\{x\in{\R}^{3}\mid\norm{x-p}<\ve\}\sub O$. 
\end{definition}
\par
Let $f:O\to\R$ be a function defined on an open set. The differetiability of $f$ at $p$ can be determined entirely from values of $f$ on $O$. This means that differetiation is a local operation. We will discuss this later.
% 1.2 Tangent Vectors
\begin{definition}
    A \hdef{tangent vector} ${v}_{p}$ is an ordered pair ${v}_{p}=(v,p)$, where $v,p\in{\R}^{3}$. Here $v$ is called the \hdef{vector part} and $p$ is called its \hdef{point of application}. Two tangent vectors are said to be \hdef{parallel} if they have the same vector part and different points of application.
\end{definition}
\begin{definition}
    Let $p\in{\R}^{3}$. The \hdef{tangent space} at $p$, denoted ${T}_{p}({\R}^{3})$, is the set of all tangent vectors that have $p$ as point of application.
\end{definition}
\par
Fix a tangent space ${T}_{p}({\R}^{3})$ and let ${T}_{p}({\R}^{3})$ adapt the operations from ${\R}^{3}\times{\R}^{3}$. We have a natural linear map $f:{T}_{p}({\R}^{3})\to{\R}^{3}$ defined by ${v}_{p}\to v$ and it is trivially an isomorphism.
\begin{definition}
    A \hdef{vector field} $V$ on ${\R}^{3}$ is a function $V:{\R}^{3}\to{\R}^{3}$ such that for all $p\in{\R}^{3}$, $V(p)\sub{T}_{p}({\R}^{3})$.
\end{definition}
\par
Let $V$ and $W$ be vector field. Let $f$ be a real-valued function. For all $p\in{\R}^{3}$, define $V+W$ by $(V+W)(p)=V(p)+W(p)$ and $(fV)(p)=f(p)V(p)$.
\begin{definition}
    Let ${U}_{1}$, ${U}_{2}$, and ${U}_{3}$ be vector fields on ${\R}^{3}$ such that ${U}_{1}(p)={(1,0,0)}_{p}$, ${U}_{2}(p)={(0,1,0)}_{p}$, and ${U}_{3}(p)={(0,0,1)}_{p}$ for all $p\in{\R}^{3}$. We call $({U}_{1},{U}_{2},{U}_{3})$ the \hdef{natural frame field} on ${\R}^{3}$.
\end{definition}
\begin{proposition}
    Let $V$ be a vector field on ${\R}^{3}$. There are three uniquely determined real-valued functions ${v}_{1}$, ${v}_{2}$, and ${v}_{3}$ on ${\R}^{3}$ such that $V={v}_{1}{U}_{1}+{v}_{2}{U}_{2}+{v}_{3}{U}_{3}$.
\end{proposition}
\begin{proof}
    For all $p\in{\R}^{3}$, $V(p)={({v}_{1}(p),{v}_{2}(p),{v}_{3}(p))}_{p}={v}_{1}(p){(1,0,0)}_{p}+{v}_{2}(p){(0,1,0)}_{p}+{v}_{3}(p){(0,0,1)}_{p}={v}_{1}(p){U}_{1}(p)+{v}_{2}(p){U}_{2}(p)+{v}_{3}{U}_{3}(p)$, hence $V=\sum{v}_{i}{U}_{i}$.
\end{proof}
\par
The functions ${v}_{1}$, ${v}_{2}$, and ${v}_{3}$ are called the \hdef{Euclidean coordinate functions} on $V$.
\begin{definition}
    A vector field $V$ is \hdef{differentiable} if its Euclidean coordinate functions are differentiable.
\end{definition}
% 1.3 Directional Derivatives
\begin{definition}
    Let $f$ be a differentiable real-valued function on ${\R}^{3}$ and let ${v}_{p}$ be a tangent vector on ${\R}^{3}$. The \hdef{directional derivative} of $f$ with respect to ${v}_{p}$, denoted ${v}_{p}[f]$, is defined to be $(\d/\d t)f(p+tv)$ at $t=0$.
\end{definition}
\begin{remark}
    We will not write the restriction every time for convenience.
\end{remark}
\begin{proposition}
    Let ${v}_{p}={({v}_{1},{v}_{2},{v}_{3})}_{p}$ be a tangent vector, then ${v}_{p}[f]=\sum{v}_{i}(\pa f/\pa{x}_{i})(p)$.
\end{proposition}
\begin{proof}
    Let $p=({p}_{1},{p}_{2},{p}_{3})$. Then ${v}_{p}[f]=(\d/\d t)f(p+tv){\vert}_{t=0}=\sum(\pa f/\pa z)(p)\cdot(\d/\d t)({p}_{i}+t{v}_{i})=\sum(\pa f/\pa{x}_{i})(p){v}_{i}$.
\end{proof}
\begin{example}
    Consider $f={x}^{2}yz$ with $p=(1,1,0)$ and $v=(1,0,-3)$. By the definition, $p+tv=(1+t,1,-3t)$, so ${v}_{p}[f]=(\d/\d t)(-3{t}^{3}-6{t}^{2}-3t)=-3$. Since $(\pa f/\pa x)=2xyz$, $(\pa f/\pa y)={x}^{2}z$, and $(\pa f/\pa z)={x}^{2}y$, we have $(\pa f/\pa x)(p)=(\pa f/\pa y)(p)=0$ and $(\pa f/\pa z)(p)=1$, so ${v}_{p}[f]=-3$.
\end{example}
\begin{proposition}
    Let $f$ and $g$ be functions on ${\R}^{3}$. Let ${v}_{p}$ and ${w}_{p}$ be tangent vectors. For all $a,b\in\R$, the following properties hold.
    \begin{enumerate}
        \item $(a{v}_{p}+b{w}_{p})[f]=a{v}_{p}[f]+b{w}_{p}[f]$.
        \item ${v}_{p}[af+bg]=a{v}_{p}[f]+b{v}_{p}[g]$.
        \item ${v}_{p}[fg]={v}_{p}[f]g(p)+f(p){v}_{p}[g]$.
    \end{enumerate}
\end{proposition}
\begin{proof}
    (\rom1) We have $(a{v}_{p}+b{w}_{p})[f]=\sum(a{v}_{i}+b{w}_{i})(\pa f/\pa{x}_{i})(p)=\sum a{v}_{i}(\pa f/\pa{x}_{i})+\sum b{w}_{i}(\pa f/\pa{x}_{i})(p)=a{v}_{p}[f]+b{w}_{p}[f]$. (\rom2) We have ${v}_{p}[af+bg]=\sum{v}_{i}(\pa(af+bg)/\pa{x}_{i})(p)=\sum{v}_{i}(\pa(af)/\pa{x}_{i})(p)+\sum{v}_{i}(\pa(bg)/\pa{x}_{i})(p)=a{v}_{p}[f]+b{v}_{p}[g]$. (\rom3) We have ${v}_{p}[fg]=\sum{v}_{i}(\pa(fg)/\pa{x}_{i})(p)=\sum{v}_{i}(\pa f/\pa{x}_{i})(p)g(p)+f(p)\sum{v}_{i}(\pa g/\pa{x}_{i})(p)={v}_{p}[f]g(p)+f(p){v}_{p}[g]$.
\end{proof}
\par
Let $V$ be a vector field, we define $V[f]$ at $p\in{\R}^{3}$ to be $V(p)[f]$. By the convention, ${U}_{i}(p)[f]=(\pa f/\pa{x}_{i})(p)$.
\begin{proposition}
    Let $V$ and $W$ be vector fields. Let $f$, $g$, and $h$ be real-valued functions. For all $a,b\in\R$, the following properties hold.
    \begin{enumerate}
        \item $(fV+gW)[h]=fV[h]+gW[h]$.
        \item $V[af+bg]=aV[f]+bV[g]$.
        \item $V[fg]=V[f]g+fV[g]$.
    \end{enumerate}
\end{proposition}
\begin{proof}
    (\rom1) For all $p\in{\R}^{3}$, $(fV+gW)(p)[h]=(f(p)V(p)+g(p)W(p))[h]=fV[h]+gW[h]$. (\rom2) For all $p\in{\R}^{3}$, $V(p)[af+bg]=aV(p)[f]+bV(p)[g]$. (\rom3) For all $p\in{\R}^{3}$, $V(p)[f]g(p)+f(p)V(p)[g]=V[f](p)g(p)+f(p)V[g](p)=(V[f]g+fV[g])(p)$.
\end{proof}
\begin{example}
    Let $V=x{U}_{1}-{y}^{2}{U}_{3}$ and let $f={x}^{2}y+{z}^{3}$. Then $V[f]=x{U}_{1}[{x}^{2}y]+x{U}_{1}[{z}^{3}]-{y}^{2}{U}_{3}[{x}^{2}y]-{y}^{2}{U}_{3}[{z}^{3}]=2{x}^{2}y-3{y}^{2}{z}^{2}$.
\end{example}
% 1.4 Curves in {\R}^{3}
\par
Let $I\sub\R$ be an open interval. Let $\al:I\to{\R}^{3}$ be a function. We can rewrite $\al(t)$ as $({\al}_{1}(t),{\al}_{2}(t),{\al}_{3}(t))$, where ${\al}_{i}:I\to\R$. We say $\al$ is \hdef{differentiable} if ${\al}_{i}$ are differentiable.
\begin{definition}
    A \hdef{curve} in ${\R}^{3}$ is a differentiable function $\al:I\to{\R}^{3}$, where $I\sub\R$ is an open interval.
\end{definition}
\begin{example}
    A curve $\al:\R\to{\R}^{3}$ defined by $\al(t)=p+tq$, where $\al(0)=p$ and $q\ne 0$, is called a \hdef{straight line}.
\end{example}
\begin{example}
    Here are some examples of curves.
    \begin{enumerate}
        \item The cruve $\al:\R\to{\R}^{3}$ defined by $\al(t)=(a\cos t,a\sin t,bt)$.
        \item The cruve $\al:\R\to{\R}^{3}$ defined by $\al(t)=(1+\cos t,\sin t,2\sin(t/2))$.
        \item The cruve $\al:\R\to{\R}^{3}$ defined by $\al(t)=({e}^{t},{e}^{-t},\sqrt{2}t)$.
        \item The cruve $\al:\R\to{\R}^{3}$ defined by $\al(t)=(3t-{t}^{3},3{t}^{2},3t+{t}^{3})$.
    \end{enumerate}
\end{example}
\begin{definition}
    Let $\al:I\to{\R}^{3}$ be a curve with $\al=({\al}_{1},{\al}_{2},{\al}_{3})$. For all $t\in I$, the \hdef{velocity vector} of $\al$ at $t$ is the tangent vector $\al'(t)={((\d{\al}_{1}/\d t)(t),(\d{\al}_{2}/\d t)(t),(\d{\al}_{3}/\d t)(t))}_{\al(t)}$ at the point $\al(t)\in{\R}^{3}$. The curve $\al$ is said to be \hdef{regular} if ${\al}_{i}\ne 0$ for all $i$.
\end{definition}
\par
Consider the velocity vector $\al'(t)$, we can rewrite it by the natural frame fields, so $\al'(t)=\sum(\d{\al}_{i}/\d t)(t){U}_{i}(\al(t))$.
\begin{definition}
    Let $\al:I\to{\R}^{3}$ be a curve and let $h:J\to I$ be differentiable, where $J$ is an open interval of $\R$. The \hdef{reparametrization} of $\al$ by $h$ is the composition $\al\comp h:J\to{\R}^{3}$.
\end{definition}
\par
The composition of differentiable functions is differentiable, so any reparametrization is differentiable, which means it is a curve.
\begin{proposition}
    Let $\be$ be the reparametrization of $\al$ by $h$, then $\be'(s)=(\d h/\d s)(s)\al'(h(s))$.
\end{proposition}
\begin{proof}
    Rewrite $\be(s)=\al(h(s))$, then we have $\be'(s)={(\d({\al}_{i}{h}_{i})/\d s)(s)}_{\al(h(s))}={(\d{\al}_{i}/\d s)(h(s))\cdot(\d h/\d s)(s)}_{\al(h(s))}=(\d h/\d s)(s)\al'(h(s))$.
\end{proof}
\begin{proposition}
    Let $\al$ be a curve and let $f$ be a differentiable function on ${\R}^{3}$, then $\al'(t)[f]=(\d(f\al)/\d t)(t)$.
\end{proposition}
\begin{proof}
    We have $\al'(t)[f]=\sum(\d{\al}_{i}/\d t)(t)\cdot(\pa f/\pa{x}_{i})(\al(t))=(\d(f\al)/\d t)(t)$ by the chain rule.
\end{proof}
\par
Now we show a general idea of parametrizations. The proofs will be included in other sections when we have enough tools. Assume every result is correct for now.
% 1.5 1-Forms
\begin{definition}
    A \hdef{1-form} $\vp$ on ${\R}^{3}$ is a function $\vp:{\Cp}_{p\in{\R}^{3}}{T}_{p}({\R}^{3})\to\R$ such that for all $a,b\in\R$ and $v,w\in{T}_{p}({\R}^{3})$ for some $p\in{\R}^{3}$, $\vp(av+bw)=a\vp(v)+b\vp(w)$.
\end{definition}
\par
Given a 1-form $\vp$, for any point $p$, denote the restriction $\vp{\vert}_{{T}_{p}({\R}^{3})}:{T}_{p}({\R}^{3})\to\R$ by ${\vp}_{p}$, then ${\vp}_{p}$ is linear. Let $\vp$ and $\psi$ be 1-forms. Define the addition and scalar multiplication by $(\vp+\psi)(v)=\vp(v)+\psi(v)$ and $(f\vp)({v}_{p})=f(p)\vp({v}_{p})$. Given any 1-form $\vp$ and point $p$, ${\vp}_{p}$ is a linear functional in ${T}_{p}^{*}({\R}^{3})$, the dual space of ${T}_{p}({\R}^{3})$.
\begin{definition}
    Let $\vp$ be a 1-form and let $V$ be a vector field. For all $p\in{\R}^{3}$, define $\vp(V)(p)={\vp}_{p}(V(p))$. We say $\vp$ is \hdef{differentiable} if for every differentiable vector field $V$, the function $\vp(V)$ is differentiable.
\end{definition}
\par
Now let $V$ and $W$ be vector fields, we have $\vp(fV+gW)(p)=\vp((fV+gW)(p))=\vp(fV(p)+gW(p))=(f\vp(V)+g\vp(W))(p)$. Similarly, $(f\vp+g\psi)(V)=f\vp(V)+g\psi(V)$.
\begin{definition}
    If $f:{\R}^{3}\to\R$ is differentiable. The \hdef{differential} of $f$, denoted $\d f$, is the function $\d f({v}_{p})={v}_{p}[f]$ for all tangent vectors ${v}_{p}$.
\end{definition}
\par
Let ${v}_{p},{w}_{p}\in{T}_{p}({\R}^{3})$ and let $a,b\in\R$, then $\d f(a{v}_{p}+b{w}_{p})=(a{v}_{p}+b{w}_{p})[f]=a{v}_{p}[f]+b{w}_{p}[f]=a\d f({v}_{p})+b\d f({w}_{p})$. Hence $\d f$ is a 1-form.
\begin{example}
    Consider the natural coordinate functions ${x}_{i}$. We have $\d{x}_{i}({v}_{p})={v}_{p}[{x}_{i}]=\sum{v}_{i}(\pa{x}_{i}/\pa{x}_{j})(p)={v}_{i}$.
\end{example}
\begin{proposition}
    If $\vp$ is a 1-form on ${\R}^{3}$, then $\vp=\sum{f}_{i}\d{x}_{i}$, where ${f}_{i}=\vp({U}_{i})$.
\end{proposition}
\begin{proof}
    Let ${v}_{p}\in{T}_{p}({\R}^{3})$, then $\vp({v}_{p})=\vp(\sum{v}_{i}{U}_{i}(p))=\sum{v}_{i}\vp({U}_{i}(p))=\sum{v}_{i}{f}_{i}(p)=\sum{f}_{i}(p)\d{x}_{i}({v}_{p})=(\sum{f}_{i}\d{x}_{i})({v}_{p})$, hence $\vp=\sum{f}_{i}\d{x}_{i}$.
\end{proof}
\par
The functions ${f}_{1}$, ${f}_{2}$, and ${f}_{3}$ are called the \hdef{Euclidean coordinate functions} of the 1-form $\vp$.
\begin{proposition}
    Let $f$ be a differentiable function on ${\R}^{3}$, then $\d f=\sum(\pa f/\pa{x}_{i})\d{x}_{i}$.
\end{proposition}
\begin{proof}
    Let ${v}_{p}\in{T}_{p}({\R}^{3})$, then $\d f({v}_{p})={v}_{p}[f]=\sum{v}_{i}(\pa f/\pa{x}_{i})(p)=\sum(\pa f/\pa{x}_{i})(p)\d{x}_{i}({v}_{p})=(\sum(\pa f/\pa{x}_{i})\d{x}_{i})({v}_{p})$, hence $\d f=\sum(\pa f/\pa{x}_{i})\d{x}_{i}$.
\end{proof}
\par
Let $f$ and $g$ be differentiable functions on ${\R}^{3}$, then $\d(f+g)=\sum(\pa(f+g)/\pa{x}_{i})\d{x}_{i}=\sum(\pa f/\pa{x}_{i})\d{x}_{i}+\sum(\pa g/\pa{x}_{i})\d{x}_{i}=\d f+\d g$. Now we denote the multiplication to be $fg$.
\begin{proposition}
    Let $f$ and $g$ be differentiable functions on ${\R}^{3}$, then $\d(fg)=g\d f+f\d g$.
\end{proposition}
\begin{proof}
    We have $\d(fg)=\sum(\pa(fg)/\pa{x}_{i})\d{x}_{i}=\sum((\pa f/\pa{x}_{i})g+(\pa g/\pa{x}_{i})f)\d{x}_{i}=g\d f+f\d g$.
\end{proof}
\begin{proposition}
    Let $f:{\R}^{3}\to\R$ and $h:\R\to\R$ be differentiable, then $\d(h(f))=(\d h(f)/\d x)\d f$.
\end{proposition}
\begin{proof}
    We have $\d(h(f))=\sum(\pa h(f)/\pa{x}_{i})\d{x}_{i}$, by the chain rule, $(\pa h(f)/\pa{x}_{i})\d{x}_{i}=(\d h(f)/\d f)(\pa x/\pa{x}_{i})$, so $\d(h(f))=(\d f(h)/\d f)\d f$.
\end{proof}
\begin{example}
    Consider the function $f=({x}^{2}-1)y+({y}^{2}+2)z$. We have $\d f=\d(({x}^{2}-1)y)+\d(({y}^{2}+2)z)=y\d({x}^{2}-1)+({x}^{2}+1)\d y+z\d({y}^{2}+2)+({y}^{2}+2)\d z=2xy\d x+({x}^{2}+2yz-1)\d y+({y}^{2}+2)\d z$. Since ${v}_{p}[f]=\d f({v}_{p})$, ${v}_{p}[f]=2{p}_{1}{p}_{2}{v}_{1}+({p}_{1}^{2}+2{p}_{2}{p}_{3}-1){v}_{2}+({p}_{2}^{2}+2){v}_{3}$.
\end{example}
% 1.6 Differential Forms
\begin{definition}
    Let $V$ be the vector space ${\R}^{3}$ and denote the space of all $p$-linear forms on $V$ by ${\LA}^{p}({V}^{*})$. Every element of ${\LA}^{p}$ is called a \hdef{p-form}. Define the \hdef{wedge product} to be a function $\wedge:{\LA}^{a}({V}^{*})\times{\LA}^{b}({V}^{*})\to{\LA}^{a+b}({V}^{*})$ such that for $\om\in{\LA}^{m}({V}^{*})$, $\eta\in{\LA}^{n}({V}^{*})$, and ${v}_{1},\dots,{v}_{m+n}\in V$, the following properties hold.
    \begin{enumerate}
        \item $(\om\wedge\eta)({v}_{1},\dots,{v}_{m+n})=({\sum}_{\si\in{\Sg}_{m+n}}\sgn(\si)\om({v}_{\si(1)},\dots,{v}_{\si(m)})\eta({v}_{\si(m+1)},\dots,{v}_{\si(m+n)}))/(m!n!)$.
        \item $\om\wedge\eta={(-1)}^{mn}\eta\wedge\om$.
    \end{enumerate}
\end{definition}
\par
Generally, a $p$-form is of the form $\sum f(x,y,z)\d{x}^{i}\wedge\cdots\d{y}^{j}\wedge\cdots\d{z}^{k}\wedge\cdots$. We have $\d{x}_{i}\wedge\d{x}_{j}=-\d{x}_{j}\wedge\d{x}_{i}$. If $i=j$, then $\d{x}_{i}\wedge\d{x}_{i}=-\d{x}_{i}\wedge\d{x}_{i}$, so $\d{x}_{i}\wedge\d{x}_{i}=0$. It is trivial that $\wedge$ is bilinear and associative, that is,
\begin{enumerate}
    \item for ${\om}_{1},{\om}_{2}\in{\LA}^{m}({V}^{*})$, $\eta\in{\LA}^{n}({V}^{*})$, and $a,b\in\R$,$(a{\om}_{1}+b{\om}_{2})\wedge\eta=a({\om}_{1}\wedge\eta)+b({\om}_{2}\wedge\eta)$ and $\eta\wedge(a{\om}_{1}+b{\om}_{2})=a(\eta\wedge{\om}_{1})+b(\eta\wedge{\om}_{2})$;
    \item for $\om\in{\LA}^{m}({V}^{*})$, $\eta\in{\LA}^{n}({V}^{*})$, and $\theta\in{\LA}^{l}({V}^{*})$, $\om\wedge(\eta\wedge\theta)=(\om\wedge\eta)\wedge\theta$.
\end{enumerate}
Now given a space of $p$-forms ${\LA}^{p}({V}^{*})$ with basis $\{{e}_{1},{e}_{2},{e}_{3}\}$, the basis of its dual space is denoted by $\{{e}^{1},{e}^{2},{e}^{3}\}$. The basis of ${\LA}^{k}({V}^{*})$ is of the form ${e}^{{i}_{1}}\wedge\cdots\wedge{e}^{{i}_{k}}$, where $1\le{i}_{1}\le\cdots\le{i}_{k}\le 3$. In this case, the dimension of ${\LA}^{p}({V}^{*})$ is $3!/(p!(3-p)!)$. If $p>4$, then $\dim({\LA}^{p}({V}^{*}))=0$, so there are no $p$-forms on ${\R}^{3}$ if $p\ge 4$.
\begin{example}
    Let $\vp=x\d x-y\d y$, $\psi=z\d x+x\d z$, $\theta=z\d y$, and $\eta=y\d x\wedge\d z+x\d y\wedge\d z$.
    \begin{enumerate}
        \item $\vp\wedge\psi=xz\d x\wedge\d x+{x}^{2}\d x\wedge\d z-yz\d y\wedge\d x-yx\d y\wedge\d z=yz\d x\wedge\d y+{x}^{2}\d x\wedge\d z-yx\d y\wedge\d z$
        \item $\theta\wedge(\vp\wedge\psi)=y{z}^{2}\d x\wedge(\d y\wedge\d y)+{x}^{2}z\d x\wedge\d z\wedge\d y-xyz\d y\wedge\d z\wedge\d y=-{x}^{2}z\d x\wedge\d y\wedge\d z$
        \item $\vp\wedge\eta=xy\d x\wedge\d x\wedge\d z+{x}^{2}\d x\wedge\d y\wedge\d z-{y}^{2}\d y\wedge\d x\wedge\d z-xy\d y\wedge\d y\wedge\d z=({x}^{2}+{y}^{2})\d x\wedge\d y\wedge\d z$
    \end{enumerate}
\end{example}
\begin{proposition}
    Let $\vp$ and $\psi$ be 1-forms, then $\vp\wedge\psi=-\psi\wedge\vp$.
\end{proposition}
\begin{proof}
    Rewrite $\vp=\sum{f}_{i}\d{x}_{i}$ and $\psi=\sum{g}_{i}\d{x}_{i}$, then $\vp\wedge\psi=\sum{f}_{i}{g}_{i}\d{x}_{i}\d{x}_{j}=\sum-{g}_{i}{f}_{i}\d{x}_{j}\d{x}_{i}=-\psi\wedge\vp$.
\end{proof}
\begin{definition}
    Let $\vp=\sum{f}_{i}\d{x}_{i}$ be a 1-form on ${\R}^{3}$. The \hdef{exterior derivative} of $\vp$ is the 2-form $\d\vp=\sum\d{f}_{i}\wedge\d{x}_{i}$. Let $\psi=\sum{f}_{i,j}\d{x}_{i}\wedge\d{x}_{j}$ be a 2-form. The \hdef{exterior derivative} of $\psi$ is the 3-form $\d\psi=\sum\d{f}_{i,j}\wedge\d{x}_{i}\wedge\d{x}_{j}$. 
\end{definition}
\par
Let $a,b\in\R$. Let $\vp=\sum{f}_{i}\d{x}_{i}$ and $\psi=\sum{g}_{i}\d{x}_{i}$ be 1-forms. Then $\d(a\vp+b\psi)=\d(\sum(a{f}_{i}+b{g}_{i})\d{x}_{i})=\sum\d(a{f}_{i}+b{g}_{i})\wedge\d{x}_{i}$, since the differential is linear, the exterior derivative is linear.
\begin{proposition}
    Let $f,g:{\R}^{3}\to\R$ be functions and let $\vp$ and $\psi$ be 1-forms. Then $\d(f\vp)=\d f\wedge\vp+f\d\vp$ and $\d(\vp\wedge\psi)=\d\vp\wedge\psi-\vp\wedge\d\psi$.
\end{proposition}
\begin{proof}
    (\rom1) Let $\vp=\sum{g}_{i}\d{x}_{i}$, then $f\vp=\sum f{g}_{i}\d{x}_{i}$, so $\d(f\vp)=\sum(f\d{g}_{i}+{g}_{i}\d f)\wedge\d{x}_{i}=\sum f\d{g}_{i}\wedge\d{x}_{i}+\sum{g}_{i}\d f\wedge\d{x}_{i}=f\d\vp+\d f\wedge\vp$. (\rom2) Since $\d{x}_{i}\wedge\d{x}_{i}=0$, without lose of generality, let $\vp=f\d x$ and let $\psi=g\d y$. Then $\d(\vp\wedge\psi)=\d(fg\d x\wedge\d y)=\d(fg)\wedge\d x\wedge\d y=(f\d g+g\d f)\wedge\d x\wedge\d y=f\d g\wedge\d x\wedge\d y+g\d f\wedge\d x\wedge\d y$. For the right hand side, $\d\vp\wedge\psi=\d f\wedge\d x\wedge g\d y=g\d f\wedge\d x\wedge\d y$ and $\vp\wedge\d\psi=f\d x\wedge\d g\wedge\d y=-f\d g\wedge\d x\wedge\d y$, hence $\d(\vp\wedge\psi)=\d\vp\wedge\psi-\vp\wedge\d\psi$.
\end{proof}
% 1.7 Mappings
\begin{definition}
    Let $F:{\R}^{n}\to{\R}^{m}$ and let ${f}_{1},\dots,{f}_{m}:{\R}^{n}\to\R$ such that $F(p)=({f}_{1}(p),\dots,{f}_{m}(p))$ for all $p\in{\R}^{n}$. The functions ${f}_{i}$ are called the \hdef{Euclidean coordinate functions} of $F$ and we denote $F=({f}_{1},\dots,{f}_{m})$.
\end{definition}
\begin{definition}
    Let $F:{\R}^{n}\to{\R}^{m}$ and $F=({f}_{1},\dots,{f}_{m})$, we say $F$ is \hdef{differentiable} if all ${f}_{i}$ are differentiable. If $F$ is differentiable, we say $F$ is a \hdef{mapping} from ${\R}^{n}$ to ${\R}^{m}$.
\end{definition}
\begin{definition}
    Let $\al:I\to{\R}^{n}$ be a curve and let $F:{\R}^{n}\to{\R}^{m}$ be a mapping. Then the composite function $\be=F(\al):I\to{\R}^{m}$ is a curve in ${\R}^{m}$ called the \hdef{image} of $\al$ under $F$.
\end{definition}
\begin{example}
    
\end{example}
\begin{definition}
    Let $F:{\R}^{n}\to{\R}^{m}$ be a mapping and let ${v}_{p}\in{T}_{p}({\R}^{n})$. The \hdef{tangent map} of $F$, denoted ${F}_{*}(v)$, is defined to be $(\d/\d t)F(p+tv)$ at $t=0$.
\end{definition}
\begin{proposition}
    Let $F=({f}_{1},\dots,{f}_{m}):{\R}^{n}\to{\R}^{m}$ be a mapping. If ${v}_{p}\in{T}_{p}({\R}^{n})$, then ${F}_{*}({v}_{p})=(v[{f}_{1}],\dots,v[{f}_{m}])$ at $F(p)$.
\end{proposition}
\begin{proof}
    Let 
\end{proof}
\begin{theorem}
    Let $F:{\R}^{n}\to{\R}^{n}$ be a mapping. If ${F}_{*p}$ is injective at some $p\in{\R}^{n}$, then there exists an open set ${U}_{p}$ containing $p$ such that $F{\vert}_{{U}_{p}}:{U}_{p}\to V$, where $V$ is open,  
\end{theorem}
\input{Ch2.tex}
\input{ExPf.tex}
\hindex
\end{document}